compiler/backend/proofs/source_to_flatProofScript.sml
@@ -1872,7 +1872,7 @@ val compile_exp_correct' = Q.prove (
     `~ st2.fp_state.canOpt`
       by (imp_res_tac fpSemPropsTheory.evaluate_fp_opts_inv >> fs[]) >>
     fs[] >>
-    qpat_x_assum `_ = (_, _)` mp_tac
+    qpat_x_assum `_ = (_, _)` mp_tac >>
     BasicProvers.TOP_CASE_TAC >>
     BasicProvers.TOP_CASE_TAC >>
     fs [] >>
@@ -1910,7 +1910,7 @@ val compile_exp_correct' = Q.prove (
     TRY (irule v_rel_FP_BoolTree) >>
     irule v_rel_weak >>
     qexists_tac `genv with v := s2.globals` >>
-    rw [subglobals_refl]))
+    rw [subglobals_refl])
   >- ( (* logical operation *)
     fs[markerTheory.Abbrev_def]>>
     qpat_x_assum`_ ⇒ _`mp_tac >>
@@ -2145,7 +2145,9 @@ val compile_exp_correct' = Q.prove (
     >- metis_tac [LENGTH_MAP])
   >- (Cases_on`l`>>fs[evaluate_def,compile_exp_def])
   >- (
-
+    (* needs invariant that we do not optimize anymore *)
+    cheat)
+  >- (
     fs [env_all_rel_cases, s_rel_cases] >>
     rw [] >>
     irule v_rel_weak >>
@@ -2172,7 +2174,7 @@ val compile_exp_correct' = Q.prove (
       simp[Once env_all_rel_cases] >> strip_tac >>
       simp [v_rel_eqns] >>
       disch_then (qspec_then `comp_map with v := bind_locals ts locals comp_map.v` mp_tac) >>
-      impl_tac >- fs [v_rel_eqns] >>
+      impl_tac >- (fs [v_rel_eqns] >> (* TODO: cannot optimise here *) cheat) >>
       strip_tac >>
       qmatch_assum_abbrev_tac`match_result_rel _ _ _ mm` >>
       Cases_on`mm`>>full_simp_tac(srw_ss())[match_result_rel_def] >>
@@ -2199,7 +2201,7 @@ val compile_exp_correct' = Q.prove (
     simp[Once env_all_rel_cases] >> strip_tac >>
     simp [v_rel_eqns] >>
     disch_then (qspec_then `comp_map with v := bind_locals ts locals comp_map.v` mp_tac) >>
-    impl_tac >- fs [v_rel_eqns] >>
+    impl_tac >- (fs [v_rel_eqns] >> (* TODO: cannot optimise here *) cheat) >>
     strip_tac >>
     qmatch_assum_abbrev_tac`match_result_rel _ _ _ mm` >>
     Cases_on`mm`>>full_simp_tac(srw_ss())[match_result_rel_def] >>
@@ -3289,7 +3291,7 @@ val compile_decs_correct' = Q.prove (
       simp [] >>
       fs [s_rel_cases] >>
       fs [v_rel_eqns] >>
-      rfs []) >>
+      rfs [] >> cheat (* no opts allowed *)) >>
     Cases_on `pmatch env.c st'.refs p answer [] ` >>
     fs []
     >- ( (* No match *)
