compiler/backend/source_to_flatScript.sml
@@ -170,7 +170,7 @@ val compile_exp_def = tDefine"compile_exp"`
     let t' = if t = None then t else SourceLoc st.row st.col en.row en.col in
       compile_exp t' env e) ∧
   (* remove FPOptimise annotations *)
-  (compile_exp t env (FpOptimise sc e) = compile_exp t env e /\
+  (compile_exp t env (FpOptimise sc e) = compile_exp t env e) /\
   (compile_exps t env [] = []) ∧
   (compile_exps t env (e::es) =
      compile_exp t env e :: compile_exps t env es) ∧
